examples/Relations.dfy
@@ -29,4 +29,5 @@ module RelationsExamples {
   lemma BuiltInIntEqIsEquivalenceRelation()
     ensures EquivalenceRelation((x: int, y: int) => (x == y))
   {}
+
 }
