src/Collections/Sets/Sets.dfy
@@ -14,10 +14,12 @@
  *******************************************************************************/
 
 include "../../Functions.dfy"
+include "../../Relations.dfy"
 
 module {:options "-functionSyntax:4"} Sets {
 
   import opened Functions
+  import opened Relations
 
   /* If all elements in set x are in set y, x is a subset of y. */
   lemma LemmaSubset<T>(x: set<T>, y: set<T>)
@@ -191,6 +193,38 @@ module {:options "-functionSyntax:4"} Sets {
     }
     assert x <= range;
     LemmaSubsetSize(x, range);
+  }
+
+ /* Any totally ordered set contains a unique minimal element. */
+  lemma LemmaUniqueMinimum<T(!new)>(R: (T, T) -> bool, s: set<T>) returns (m: T)
+    requires |s| > 0 && TotalOrdering(R)
+    ensures IsMinimum(R, m, s) && (forall n: T | IsMinimum(R, n, s) :: m == n)
+  {
+    var x :| x in s;
+    if s == {x} {
+      m := x;
+    } else {
+      var m' := LemmaUniqueMinimum(R, s - {x});
+      if
+      case R(m', x) => m := m';
+      case R(x, m') => m := x;
+    }
+  }
+
+  /* Any totally ordered set contains a unique maximal element. */
+  lemma LemmaUniqueMaximum<T(!new)>(R: (T, T) -> bool, s: set<T>) returns (m: T)
+    requires |s| > 0 && TotalOrdering(R)
+    ensures IsMaximum(R, m, s) && (forall n: T | IsMaximum(R, n, s) :: m == n)
+  {
+    var x :| x in s;
+    if s == {x} {
+      m := x;
+    } else {
+      var m' := LemmaUniqueMaximum(R, s - {x});
+      if
+      case R(m', x) => m := x;
+      case R(x, m') => m := m';
+    }
   }
 
 }
